src/Lustre/Denot/Kenv.v
@@ -1,0 +1,36 @@
+Require Import Cpo.
+
+(** * Environment types of the Kahn semantics *)
+
+Section KENV.
+
+  (** identifier of variables *)
+  Context {ident : Type}.
+
+  Inductive key :=
+  | Var : ident -> key
+  | Last : ident -> key.
+
+  Definition env (A : Type) : cpo := DS_prod (fun _:key => A).
+
+  (** apply a function to every stream of the environment *)
+  Definition ext_env {A B : Type} : (DS A -C-> DS B) -C-> (env A -C-> env B).
+    apply curry, Dprodi_DISTR; intro i.
+    refine ((AP _ _ @2_ FST _ _) (PROJ _ i @_ SND _ _)).
+  Defined.
+
+  Lemma ext_env_simpl : forall A B f env i,
+      @ext_env A B f env i = f (env i).
+  Proof.
+    trivial.
+  Qed.
+
+  (** state/branch identifier *)
+  Context {id_st : Type}.
+
+  Context {id_st_dec : forall i j : id_st, { i = j } + { ~ i = j }}.
+
+  Definition id_st_eqb (i j : id_st) : bool :=
+    match id_st_dec i j with left _ => true | _ => false end.
+
+End KENV.
